Envasar

CODIGO/SUMA/Problems/Envasar.dfy
@@ -9,18 +9,58 @@ ghost predicate Envasar(A:multiset<nat>, E:nat, k:nat)
 { 
   exists I:multiset<multiset<nat>> :: 
    && |I| <= k 
-   && Union(I) == A
+   && GUnion(I) == A
    && forall e | e in I :: (e <= A && GSumNat(e) <= E)
     
 }
 
-ghost function Union (I:multiset<multiset<nat>>) : multiset<nat>
+
+function minMultiset (m:multiset<multiset<nat>>): (l:multiset<nat>)
+requires m != multiset{}
+ensures l in m && (forall x | x in m :: GSumNat(l) <= GSumNat(l)) 
+
+// UNION
+
+ghost function GUnion (I:multiset<multiset<nat>>) : multiset<nat>
 {
   if I == multiset{} then multiset{}
-  else var i :| i in I; i + Union(I-multiset{i})
+  else var i :| i in I; i + GUnion(I-multiset{i})
 }
 
+function FUnion (I:multiset<multiset<nat>>) : multiset<nat>
+{
+  if I == multiset{} then multiset{}
+  else var i := minMultiset(I); i + FUnion(I-multiset{i})
+}
+
+lemma {:induction m} GUnionPartes(m : multiset<multiset<nat>>, x : multiset<nat>)
+ensures GUnion(m) == x + GUnion(m - multiset{x})
+
+
+lemma {:induction m} FUnionComputaGUnion(m : multiset<multiset<nat>>)
+ensures FUnion(m) == GUnion(m)
+{ 
+  if m == multiset{} {
+    assert FUnion(m) == GUnion(m);
+  }
+  else {
+    var x :| x in m;
+    FUnionComputaGUnion(m - multiset{x});
+    assert FUnion(m - multiset{x}) == GUnion(m-multiset{x});
+
+    assume FUnion(m) == x + FUnion(m-multiset{x});
+    assume x + FUnion(m) == x + GUnion(m - multiset{x});
+    assume FUnion(m) == GUnion(m);
+  }
+}
+
+// VERIFICACION
+
 method {:verify true} checkEnvasar(A:multiset<nat>, E:nat, k:nat, I:multiset<multiset<nat>>) returns (b:bool)
-ensures b ==(   |I| <= k 
-             && Union(I) == A
-             && forall e | e in I :: e <= A && GSumNat(e) <= E) 
+ensures b ==  (|I| <= k 
+             && GUnion(I) == A )
+             //&& forall e | e in I :: e <= A && GSumNat(e) <= E )
+{
+  FUnionComputaGUnion(I);
+  b := |I| <= k && FUnion(I) == A;
+}
